Fixing Linking problem

backend/Duplicate.v
@@ -34,35 +34,35 @@ Definition verify_mapping (xf: xfunction) (tc: code) (tentry: node) : res unit :
 
 (** * Entry points *)
 
-Definition transf_function (f: function) : res xfunction :=
+Definition transf_function_aux (f: function) : res xfunction :=
   let (tcte, mp) := duplicate_aux f in
   let (tc, te) := tcte in
   let xf := {| fn_RTL := (mkfunction (fn_sig f) (fn_params f) (fn_stacksize f) tc te); fn_revmap := mp |} in
   do u <- verify_mapping xf tc te;
   OK xf.
 
-Theorem transf_function_preserves:
+Theorem transf_function_aux_preserves:
   forall f xf,
-  transf_function f = OK xf ->
+  transf_function_aux f = OK xf ->
      fn_sig f = fn_sig (fn_RTL xf) /\ fn_params f = fn_params (fn_RTL xf) /\ fn_stacksize f = fn_stacksize (fn_RTL xf).
 Proof.
-  intros. unfold transf_function in H. destruct (duplicate_aux _) as (tcte & mp). destruct tcte as (tc & te). monadInv H.
+  intros. unfold transf_function_aux in H. destruct (duplicate_aux _) as (tcte & mp). destruct tcte as (tc & te). monadInv H.
   repeat (split; try reflexivity).
 Qed.
 
-Remark transf_function_fnsig: forall f xf, transf_function f = OK xf -> fn_sig f = fn_sig (fn_RTL xf).
-  Proof. apply transf_function_preserves. Qed.
-Remark transf_function_fnparams: forall f xf, transf_function f = OK xf -> fn_params f = fn_params (fn_RTL xf).
-  Proof. apply transf_function_preserves. Qed.
-Remark transf_function_fnstacksize: forall f xf, transf_function f = OK xf -> fn_stacksize f = fn_stacksize (fn_RTL xf).
-  Proof. apply transf_function_preserves. Qed.
+Remark transf_function_aux_fnsig: forall f xf, transf_function_aux f = OK xf -> fn_sig f = fn_sig (fn_RTL xf).
+  Proof. apply transf_function_aux_preserves. Qed.
+Remark transf_function_aux_fnparams: forall f xf, transf_function_aux f = OK xf -> fn_params f = fn_params (fn_RTL xf).
+  Proof. apply transf_function_aux_preserves. Qed.
+Remark transf_function_aux_fnstacksize: forall f xf, transf_function_aux f = OK xf -> fn_stacksize f = fn_stacksize (fn_RTL xf).
+  Proof. apply transf_function_aux_preserves. Qed.
 
-Definition transf_fundef_aux (f: fundef) : res xfundef :=
+Definition transf_function (f: function) : res function :=
+  do xf <- transf_function_aux f;
+  OK (fn_RTL xf).
+
+Definition transf_fundef (f: fundef) : res fundef :=
   transf_partial_fundef transf_function f.
-
-Definition transf_fundef (f: fundef): res fundef :=
-  do xf <- transf_fundef_aux f;
-  OK (fundef_RTL xf).
 
 Definition transf_program (p: program) : res program :=
   transform_partial_program transf_fundef p.
